pulse/lib/steel/pulse/Pulse.Syntax.Builder.fst
@@ -1,12 +1,17 @@
 module Pulse.Syntax.Builder
 open Pulse.Syntax
 
+let pat_var s = Pat_Var s
+let pat_const c = Pat_Constant c
+let pat_cons fv vs = Pat_Cons fv vs
+
 let tm_return ctag insert_eq term = Tm_Return { ctag; insert_eq; term }
 let tm_abs b q ascription body = Tm_Abs { b; q; ascription; body }
 let tm_stapp head arg_qual arg = Tm_STApp { head; arg_qual; arg }
 let tm_bind binder head body = Tm_Bind { binder; head; body }
 let tm_totbind _binder head body = Tm_TotBind { head; body }
 let tm_if b then_ else_ post = Tm_If { b; then_; else_; post }
+let tm_match sc returns_ brs = Tm_Match {sc; returns_; brs}
 let tm_elim_exists p = Tm_ElimExists { p }
 let tm_intro_exists erased p witnesses = Tm_IntroExists { erased; p; witnesses; should_check=should_check_true }
 let tm_while invariant condition condition_var body = Tm_While { invariant; condition; condition_var; body }
