pulse/lib/steel/pulse/Pulse.Syntax.Naming.fsti
@@ -2,6 +2,7 @@ module Pulse.Syntax.Naming
 
 open FStar.List.Tot
 open Pulse.Syntax.Base
+open Pulse.Common
 
 module L = FStar.List.Tot
 
@@ -77,6 +78,12 @@ let rec freevars_st (t:st_term)
       Set.union (Set.union (freevars b) (freevars_st then_))
                 (Set.union (freevars_st else_) (freevars_term_opt post))
 
+    | Tm_Match { sc ; returns_; brs } ->
+      let (@@) = Set.union in
+      freevars sc
+        @@ freevars_term_opt returns_
+        @@ freevars_branches brs
+
     | Tm_IntroPure { p }
     | Tm_ElimExists { p } ->
       freevars p
@@ -111,6 +118,10 @@ let rec freevars_st (t:st_term)
 
     | Tm_ProofHintWithBinders { binders; v; t } ->
       Set.union (freevars v) (freevars_st t)
+and freevars_branches (t:list (pattern & st_term)) : Set.set var =
+  match t with
+  | [] -> Set.empty
+  | (_, b)::tl -> freevars_st b `Set.union` freevars_branches tl
 
 let rec ln' (t:term) (i:int) : Tot bool (decreases t) =
   match t.t with
@@ -191,6 +202,11 @@ let rec ln_st' (t:st_term) (i:int)
       ln_st' else_ i &&
       ln_opt' post (i + 1)
   
+    | Tm_Match {sc; returns_; brs } ->
+      ln' sc i &&
+      ln_opt' returns_ i &&
+      for_all_dec t (ln_branch i) brs
+
     | Tm_IntroPure { p }
     | Tm_ElimExists { p } ->
       ln' p i
@@ -232,6 +248,15 @@ let rec ln_st' (t:st_term) (i:int)
       let n = L.length binders in
       ln' v (i + n) &&
       ln_st' t (i + n)
+
+and ln_branch (i:int) (b : pattern & st_term) : Tot bool (decreases b) =
+  let (p, e) = b in
+  match p with
+  | Pat_Cons fv l -> ln_st' e (i + length l)
+  | Pat_Constant _ -> ln_st' e i
+  | Pat_Var _ -> ln_st' e (i+1)
+  | Pat_Dot_Term None -> true
+  | Pat_Dot_Term (Some e) -> false // FIXME come back to this
 
 let ln (t:term) = ln' t (-1)
 let ln_st (t:st_term) = ln_st' t (-1)
@@ -383,6 +408,11 @@ let rec subst_st_term (t:st_term) (ss:subst)
               else_ = subst_st_term else_ ss;
               post = subst_term_opt post (shift_subst ss) }
 
+    | Tm_Match { sc; returns_; brs } ->
+      Tm_Match { sc = subst_term sc ss;
+                 returns_ = subst_term_opt returns_ ss;
+                 brs = subst_branches t ss brs }
+
     | Tm_IntroPure { p; should_check } ->
       Tm_IntroPure { p = subst_term p ss; should_check }
 
@@ -437,6 +467,24 @@ let rec subst_st_term (t:st_term) (ss:subst)
     in
     { t with term = t' }
 
+and subst_branches (t:st_term) (ss:subst) (brs : list branch{brs << t})
+: Tot (list branch) (decreases brs)
+=
+  map_dec t brs (fun br -> subst_branch ss br)
+
+and subst_branch (ss:subst) (b : pattern & st_term) : Tot (pattern & st_term) (decreases b) =
+  let (p, e) = b in
+  let pat_n_binders (p:pattern) : nat =
+    match p with
+    | Pat_Constant _ -> 0
+    | Pat_Var _ -> 1
+    | Pat_Cons _ args -> L.length args
+    | Pat_Dot_Term _ -> 0
+  in
+  let nn = pat_n_binders p in
+  let ss = shift_subst_n nn ss in
+  p, subst_st_term e ss
+
 let open_st_term' (t:st_term) (v:term) (i:index) : st_term =
   subst_st_term t [ DT i v ]
 
@@ -480,6 +528,24 @@ let close_st_term' (t:st_term) (v:var) (i:index) : st_term =
 let close_term t v = close_term' t v 0
 let close_st_term t v = close_st_term' t v 0
 let close_comp t v = close_comp' t v 0
+
+let close_term_n t vs =
+  let rec aux (i:nat) (vs:list var) (t:term) : Tot term (decreases vs) =
+    match vs with
+    | [] -> t
+    | v::vs ->
+      aux (i+1) vs (close_term' t v i)
+  in
+  aux 0 (List.rev vs) t
+
+let close_st_term_n t vs =
+  let rec aux (i:nat) (vs:list var) (t:st_term) : Tot st_term (decreases vs) =
+    match vs with
+    | [] -> t
+    | v::vs ->
+      aux (i+1) vs (close_st_term' t v i)
+  in
+  aux 0 (List.rev vs) t
 
 val close_open_inverse' (t:term) 
                         (x:var { ~(x `Set.mem` freevars t) } )
