pulse/lib/steel/pulse/Pulse.Checker.Match.fsti
@@ -1,0 +1,17 @@
+module Pulse.Checker.Match
+
+module T = FStar.Tactics.V2
+
+open Pulse.Syntax
+open Pulse.Typing
+open Pulse.Checker.Common
+
+val check_match
+        (g:env)
+        (sc:term)
+        (brs:list branch)
+        (pre:term)
+        (pre_typing: tot_typing g pre tm_vprop)
+        (post_hint:post_hint_for_env g)
+        (check:check_t)
+  : T.Tac (checker_result_t g pre (Some post_hint))
