pulse/lib/steel/pulse/Pulse.Soundness.Match.fst
@@ -1,0 +1,69 @@
+module Pulse.Soundness.Match
+
+open Pulse.Soundness.Common
+open Pulse.Syntax.Base
+open Pulse.Syntax.Pure
+open Pulse.Typing
+open Pulse.Elaborate.Core
+open Pulse.Elaborate.Pure
+module RT = FStar.Reflection.Typing
+module R = FStar.Reflection.V2
+module T = FStar.Tactics.V2
+module L = FStar.List.Tot
+
+let complete_soundness
+  (g:stt_env)
+  (#sc_u:universe)
+  (#sc_ty:term)
+  (#sc:term)
+  (brs:list branch)
+  (c:comp_st)
+  (d : brs_typing g sc_u sc_ty sc brs c)
+  (comp : pats_complete g sc sc_ty (L.map (fun (p, _) -> elab_pat p) brs))
+  (bs : list (list R.binding))
+  : RT.match_is_complete (elab_env g) (elab_term sc) (elab_term sc_ty)
+                                 (List.Tot.map fst (elab_branches d))
+                                 bs
+  = let PC_Elab _ _ _ _ bs' s = comp in
+    assume (L.map fst (elab_branches d) == L.map (fun (p, _) -> elab_pat p) brs); // FIXME
+    assume (bs == bs'); // FIXME
+    s
+
+let match_soundness
+  (g:stt_env)
+  (t:st_term)
+  (c:comp)
+  (d:st_typing g t c{T_Match? d})
+  (soundness:soundness_t d)
+  (ct_soundness: (g:stt_env -> c:comp -> uc:universe ->
+                  d':comp_typing g c uc{d' << d} ->
+              GTot (RT.tot_typing (elab_env g)
+                              (elab_comp c)
+                              (RT.tm_type uc))))
+  : GTot (RT.tot_typing (elab_env g)
+                        (elab_st_typing d)
+                        (elab_comp c))
+  =
+  let T_Match _g sc_u sc_ty sc (E sc_ty_d) (E sc_d) _c brs brs_ty brs_complete = d in
+
+  let sc_e_ty : R.typ = elab_term sc_ty in
+  let sc_e_ty_t : RT.typing (elab_env g) sc_e_ty (T.E_Total, RT.tm_type sc_u) = sc_ty_d in
+
+  let sc_e = elab_term sc in
+  let sc_e_t : RT.typing (elab_env g) sc_e (T.E_Total, sc_e_ty) = sc_d in
+
+  let brs_e : list R.branch =
+    elab_branches brs_ty
+  in
+  let rcty = (T.E_Total, elab_comp c) in
+  let PC_Elab _ _ _ _ bnds _ = brs_complete in
+  let brs_e_ty : RT.branches_typing (elab_env g) sc_u sc_e_ty sc_e rcty brs_e bnds =
+    magic ()
+  in
+  let brs_complete
+     : RT.match_is_complete (elab_env g) (elab_term sc) (elab_term sc_ty) (List.Tot.map fst brs_e) bnds
+   = assume (L.map fst (elab_branches brs_ty) == L.map fst brs_e);
+     complete_soundness g brs c brs_ty brs_complete bnds
+  in
+  assume (elab_st_typing d == R.pack_ln (R.Tv_Match sc_e None brs_e));
+  RT.T_Match _ _ _ sc_e T.E_Total sc_e_ty_t T.E_Total sc_e_t brs_e rcty bnds brs_complete brs_e_ty
