pulse/lib/steel/pulse/Pulse.Typing.FV.fst
@@ -120,6 +120,9 @@ let rec freevars_close_st_term' (t:st_term) (x:var) (i:index)
       freevars_close_st_term' else_ x i;          
       freevars_close_term_opt' post x (i + 1)      
 
+    | Tm_Match _ ->
+      admit ()
+
     | Tm_IntroPure { p } 
     | Tm_ElimExists { p } ->
       freevars_close_term' p x i
@@ -431,6 +434,9 @@ let rec st_typing_freevars (#g:_) (#t:_) (#c:_)
        vars_of_env g;
     };
     comp_typing_freevars ct
+
+    | T_Match _ _ _ _ _ _ _ _ _ _ ->
+      admit ()
 
    | T_Frame _ _ _ _ df dc ->
      tot_typing_freevars df;
